theories/FOL/Incompleteness/VR.v
@@ -4,14 +4,31 @@ From Undecidability.Shared Require Import Dec embed_nat.
 
 From Undecidability.FOL.Util Require Import Syntax_facts FullDeduction FullDeduction_facts FullTarski FullTarski_facts Axiomatisations FA_facts Syntax.
 From Undecidability.FOL Require Import PA.
-Import Vector.VectorNotations.
 
 Print prv.
+
+
+
+(* Notation for satisfying list theories *)
+Notation "I ⊨=L T" := (forall psi, List.In psi T -> I ⊨= psi) (at level 20).
+(* Notation for explicitely giving model *)
+Notation "I ; rho '⊨' phi" := (@sat _ _ _ I _ rho phi) (at level 20, rho at next level).
+
+(* increasing x instead of k to be able to use recursive formulae *)
+(* NOTE this definition requires extensionality of the model *)
+Notation "x 'i⧀' y"  := (exists k, y = (iσ x) i⊕ k) (at level 42) : PA_Notation.
+(* Overwriting notation from PA.v to be useful in any way *)
+Notation "x '⧀' y"  := (∃ y`[↑] == ((σ x`[↑]) ⊕ $0)) (at level 42) : PA_Notation.
+(* I need another oless *)
+Notation "x '⧀comm' y"  := (∃ y`[↑] == (σ $0 ⊕ x`[↑])) (at level 42) : PA_Notation.
+
 
 
 Section sigma.
   Existing Instance PA_funcs_signature.
   Existing Instance PA_preds_signature.
+
+  Existing Instance falsity_on.
 
   (* TODO need to remove ff flags from these structures to ease inductions *)
 
@@ -21,15 +38,25 @@ Section sigma.
   Inductive Δ0 : form -> Prop :=
   | Delta_fal : Δ0 ⊥
   | Delta_eq : forall t s, Δ0 (t == s)
-  (* | Delta_lt ff : forall t s, @Δ0 ff (t ⧀ s) *)
+  | Delta_lt : forall t s, Δ0 (t ⧀ s)
   | Delta_Conj : forall α β, Δ0 α -> Δ0 β -> Δ0 (α ∧ β)
   | Delta_Disj : forall α β, Δ0 α -> Δ0 β -> Δ0 (α ∨ β)
   | Delta_Impl : forall α β, Δ0 α -> Δ0 β -> Δ0 (α ~> β).
 
+  Check exist_times.
+  Fixpoint oplus_times n : term :=
+    match n with
+    | 0 => zero
+    | 1 => $0
+    | S n => oplus_times n ⊕ $n
+    end.
+
   Inductive Δ0' : form -> Prop :=
   | Delta_id : forall α, Δ0 α -> Δ0' α
-  | Delta_bounded_exist : forall α, Δ0' α -> Δ0' (∃ ($0 ⧀ $1) ∧ α)
-  | Delta_bounded_forall : forall α, Δ0' α -> Δ0' (∀ $0 ⧀ $1 ~> α).
+  | Delta_bounded_exist : forall α t, Δ0' α -> Δ0' (∃ ($0 ⧀ t`[↑]) ∧ α)
+  | Delta_bounded_exist_comm : forall α t, Δ0' α -> Δ0' (∃ ($0 ⧀comm t`[↑]) ∧ α)
+  | Delta_bounded_forall : forall α t, Δ0' α -> Δ0' (∀ $0 ⧀ t`[↑] ~> α)
+  (*| Delta_bounded_exist_times : forall α n t, Δ0' α -> Δ0' (exist_times n (oplus_times n ⧀ t`[↑]) ∧ α)*).
 
   Inductive Σ1 : form -> Prop :=
   | Sigma_Delta : forall α, Δ0' α -> Σ1 α
@@ -46,6 +73,80 @@ Section sigma.
   Lemma PNF_impl φ1 φ2 : Π1 φ1 -> Σ1 φ2 -> exists ψ, Σ1 ψ /\ Qeq ⊢C (φ1 ~> φ2) <~> ψ.
   Proof. Admitted.
 
+  Lemma exists_compression' φ : bounded 2 φ -> Δ0' φ -> exists ψ, Δ0' ψ /\ Qeq ⊢C (∃ ψ) <~> ∃∃φ.
+  Proof.
+    intros Hb Hd.
+    exists (∃ ($0 ⧀ $1) ∧ ∃ ($0 ⧀comm $2) ∧ φ).
+    split.
+    { apply (Delta_bounded_exist $0), (Delta_bounded_exist_comm $1), Hd. }
+    apply CI.
+    - apply II.
+      eapply ExE.
+      { apply Ctx; now left. }
+      cbn -[Qeq]. unfold "↑". fold ↑.
+      change (List.map (subst_form ↑) Qeq) with Qeq.
+      eapply ExE.
+      { apply Ctx; now left. }
+      cbn -[Qeq]. unfold "↑". fold ↑.
+      change (List.map (subst_form ↑) Qeq) with Qeq.
+      eapply ExE.
+      { eapply CE2, Ctx. now left. }
+      cbn -[Qeq]. unfold "↑". fold ↑.
+      change (List.map (subst_form ↑) Qeq) with Qeq.
+      eapply ExI with (t := $1). cbn -[Qeq].
+      eapply ExI with (t := $0). cbn -[Qeq].
+      eapply IE.
+      2: { eapply CE2, Ctx. now left. }
+      eapply Weak with (A := Qeq).
+      2: { intros f H. now do 4 right. }
+      apply II. rewrite !subst_comp.
+      apply Ctx. left.
+      rewrite <-subst_var at 1.
+      eapply bounded_subst.
+      + apply Hb.
+      + intros [|[|k]] H; cbn; reflexivity + lia.
+    - apply II.
+      eapply ExE.
+      { apply Ctx; now left. }
+      cbn -[Qeq]. unfold "↑". fold ↑.
+      change (List.map (subst_form ↑) Qeq) with Qeq.
+      eapply ExE.
+      { apply Ctx; now left. }
+      cbn -[Qeq]. unfold "↑". fold ↑.
+      change (List.map (subst_form ↑) Qeq) with Qeq.
+      apply Weak with (A := (φ :: Qeq)%list).
+      2: { intros ϕ [<-|H].
+           - now left.
+           - now do 3 right. }
+      apply ExI with (t := σ $1 ⊕ $0).
+      cbn -[Qeq]. unfold "↑". fold ↑.
+      apply ExI with (t := $1).
+      cbn -[Qeq]. unfold "↑". fold ↑.
+      apply CI.
+      { apply ExI with (t := $0). cbn -[Qeq].
+        eapply AllE with (t := σ $1 ⊕ $0) (phi := $0 == $0).
+        apply Ctx. right. now left. }
+
+      apply ExI with (t := $0).
+      cbn -[Qeq]. unfold "↑". fold ↑.
+      apply CI.
+      { apply ExI with (t := $1). cbn -[Qeq].
+        eapply AllE with (t := σ $1 ⊕ $0) (phi := $0 == $0).
+        apply Ctx. right. now left. }
+      rewrite !subst_comp. erewrite bounded_subst; first instantiate (1 := var).
+      + rewrite subst_var. now apply Ctx.
+      + exact Hb.
+      + intros [|[|k]] Hk; cbn; reflexivity + lia.
+  Qed.
+  Lemma exists_compression φ n : bounded n φ -> Δ0' φ ->
+                                 exists ψ, Δ0' ψ /\ Qeq ⊢C (∃ ψ) <~> exist_times n φ.
+  Proof.
+    induction n as [|n IH] in φ |-*; intros Hb Hd.
+    all: cbn [exist_times iter].
+    - exists φ[↑]. cbn [exist_times iter]. admit.
+  Admitted.
+
+
   Lemma Σcompleteness : forall φ, Σ1 φ -> interp_nat ⊨= φ -> Qeq ⊢C φ.
   Proof. Admitted. (* WIP by Marc *)
   Lemma Q_sound φ : Qeq ⊢C φ -> interp_nat ⊨= φ.
@@ -60,17 +161,6 @@ Section sigma.
   Qed.
 End sigma.
 
-
-(* Notation for satisfying list theories *)
-Notation "I ⊨=L T" := (forall psi, List.In psi T -> I ⊨= psi) (at level 20).
-(* Notation for explicitely giving model *)
-Notation "I , rho '⊨' phi" := (@sat _ _ _ I _ rho phi) (at level 20, rho at next level).
-
-(* increasing x instead of k to be able to use recursive formulae *)
-(* NOTE this definition requires extensionality of the model *)
-Notation "x 'i⧀' y"  := (exists k, y = (iσ x) i⊕ k) (at level 42) : PA_Notation.
-(* Overwriting notation from PA.v to be useful in any way *)
-Notation "x '⧀' y"  := (∃ y`[↑] == ((σ x`[↑]) ⊕ $0)) (at level 42) : PA_Notation.
 Section Qmodel.
   Existing Instance PA_funcs_signature.
   Existing Instance PA_preds_signature.
@@ -215,167 +305,406 @@ Section Qmodel.
 End Qmodel.
 
 
+Section completeness.
+  Existing Instance PA_funcs_signature.
+  Existing Instance PA_preds_signature.
+
+  Definition Qdec φ := Qeq ⊢C φ \/ Qeq ⊢C ¬φ.
+
+  Existing Instance class.
+  Existing Instance interp_nat.
+
+  Hypothesis completeness : forall φ,
+      Qeq ⊢C φ <-> forall (M : Type) (I : interp M) ρ, extensional I -> I ⊨=L Qeq -> ρ ⊨ φ.
+
+  Lemma exists_compression' φ : bounded 2 φ -> Δ0' φ -> exists ψ, Δ0' ψ /\ Qeq ⊢C (∃ ψ) <~> ∃∃φ.
+  Proof.
+    intros Hb Hd. exists (∃ ($0 ⧀ $1) ∧ ∃ ($0 ⧀ $2) ∧ φ).
+    split; first admit.
+    apply completeness. intros M I ρ Mext MQ.
+    split.
+    - admit.
+    - intros (x & y & Hxy).
+      eexists. exists x. split.
+      { cbn. exists y. rewrite Mext. reflexivity. }
+      exists y. split.
+      { cbn. exists x. admit. }
+  Abort.
+
+  Lemma dec_completeness M (I : interp M) (QM : I ⊨=L Qeq) (Mext : extensional I) ρN ρM φ :
+    Qdec φ -> interp_nat; ρN ⊨ φ <-> I; ρM ⊨ φ.
+  Proof.
+    intros [Hφ|Hφ]; rewrite completeness in Hφ; try assumption; split.
+    - intros _. now apply Hφ.
+    - intros _. apply Hφ.
+      + easy.
+      + auto using nat_is_Q_model.
+    - intros []%Hφ.
+      + easy.
+      + auto using nat_is_Q_model.
+    - now intros []%Hφ.
+  Qed.
+  Lemma sat_single_PA M (I : interp M) φ ρ k : (iμ k .: ρ) ⊨ φ <-> ρ ⊨ φ[(num k)..].
+  Proof.
+    replace (iμ k) with (eval ρ (num k)).
+    - apply sat_single.
+    - induction k; cbn; congruence.
+  Qed.
+  Lemma sat_single_nat φ ρ k : (k .: ρ) ⊨ φ <-> ρ ⊨ φ[(num k)..].
+  Proof.
+    replace k with (iμ k) at 1.
+    - now rewrite sat_single_PA.
+    - induction k; cbn; congruence.
+  Qed.
+
+  Section value_disj.
+    Variable P1 P2 : nat -> Prop.
+    Hypothesis P_disjoint : forall x, P1 x -> P2 x -> False.
+
+    Variable φ1 φ2 : form.
+    Hypothesis (φ1_bounded : bounded 2 φ1) (φ2_bounded : bounded 2 φ2).
+    Hypothesis (φ1_dec : forall x k, Qdec (φ1[num x .: (num k) ..]))
+               (φ2_dec : forall x k, Qdec (φ2[num x .: (num k) ..])).
+    Hypothesis (φ1_sem : forall x ρ, P1 x <-> interp_nat; ρ ⊨ ∃ φ1[(num x) ..])
+               (φ2_sem : forall x ρ, P2 x <-> interp_nat; ρ ⊨ ∃ φ2[(num x) ..]).
 
 
-Section value.
+    Definition φ1' := φ1 ∧ ∀ $0 ⧀ $2 ~> φ2[$1 .: $0 ..] ~> ⊥.
+    Definition φ2' := φ2 ∧ ∀ $0 ⧀ $2 ~> φ1[$1 .: $0 ..] ~> ⊥.
+
+    Lemma φ1_bounded_subst ρ : φ1[ρ] = φ1[ρ 0 .: (ρ 1) ..].
+    Proof.
+      eapply bounded_subst; first apply φ1_bounded. intros [|[|k]]; easy + lia.
+    Qed.
+    Lemma φ2_bounded_subst ρ : φ2[ρ] = φ2[ρ 0 .: (ρ 1) ..].
+    Proof.
+      eapply bounded_subst; first apply φ2_bounded. intros [|[|k]]; easy + lia.
+    Qed.
+
+    Lemma φ1'_bounded : bounded 2 φ1'.
+    Proof using φ1_bounded.
+      solve_bounds.
+      - assumption.
+      - cbn. unfold "↑". constructor. lia.
+      - cbn. unfold "↑". constructor.
+        admit.
+      - eapply subst_bound; first eassumption.
+        intros [|[|n]] H.
+        + constructor. lia.
+        + constructor. lia.
+        + lia.
+    Admitted.
+
+    Lemma φ1_sem' x ρ : P1 x <-> exists k, interp_nat; ρ ⊨ φ1[num x .: (num k) ..].
+    Proof.
+      rewrite φ1_sem. cbn.
+      setoid_rewrite sat_single_nat. setoid_rewrite subst_comp.
+      setoid_rewrite φ1_bounded_subst. cbn.
+      setoid_rewrite num_subst. reflexivity.
+    Qed.
+    Lemma φ2_sem' x ρ : P2 x <-> exists k, interp_nat; ρ ⊨ φ2[num x .: (num k) ..].
+    Proof.
+      rewrite φ2_sem. cbn.
+      setoid_rewrite sat_single_nat. setoid_rewrite subst_comp.
+      setoid_rewrite φ2_bounded_subst. cbn.
+      setoid_rewrite num_subst. reflexivity.
+    Qed.
+
+    Lemma DR1 x : P1 x -> Qeq ⊢C ∃ φ1'[(num x)..].
+    Proof.
+      intros H. apply completeness. intros M I ρ Mext QM.
+      assert (exists k, (fun _ => 0) ⊨ φ1[num x .: (num k) ..]) as [k Hk] by now apply φ1_sem'.
+      exists (iμ k). split.
+      - rewrite sat_single_PA, subst_comp, φ1_bounded_subst. cbn.
+        rewrite num_subst. eapply dec_completeness; eauto.
+      - cbn. intros k' [d Hd] H2.
+
+        assert (standard k') as [k'' <-].
+        { unshelve eapply standard_le; try auto. exists d. now apply Mext. }
+
+        rewrite !sat_single_PA, !subst_comp, φ2_bounded_subst in H2. cbn in H2.
+        rewrite !num_subst in H2.
+
+        enough (P2 x) by (eapply P_disjoint; eassumption).
+        eapply φ2_sem' with (ρ := fun _ => 0). exists k''. eapply dec_completeness; eauto.
+    Qed.
+    Lemma DR2 x : P2 x -> Qeq ⊢C ¬∃ φ1'[(num x)..].
+    Proof.
+      intros H. apply completeness. intros M I ρ Mext QM [k [Hk1 Hk2]].
+      cbn in Hk1, Hk2. cbn.
+      assert (exists k, (fun _ => 0) ⊨ φ2[num x .: (num k) ..]) as [kk Hkk] by now apply φ2_sem'.
+      apply (Hk2 (iμ kk)).
+      - enough (~standard k).
+        { setoid_rewrite Mext. apply nonstandard_large; assumption. }
+        intros [k' <-].
+
+        rewrite sat_single_PA in Hk1. rewrite !subst_comp, φ1_bounded_subst in Hk1. cbn in Hk1.
+        rewrite num_subst in Hk1.
+
+        enough (P1 x) by (eapply P_disjoint; eassumption).
+        eapply φ1_sem' with (ρ := (fun _ => 0)). exists k'. eapply dec_completeness; eauto.
+      - rewrite sat_single_PA, !subst_comp, φ2_bounded_subst. cbn.
+        rewrite !num_subst. eapply dec_completeness; eauto.
+    Qed.
+  End value_disj.
+
+  Section value.
+
+    Variable f : nat -> nat -> Prop.
+    Hypothesis f_func : forall x y1 y2, f x y1 -> f x y2 -> y1 = y2.
+
+    Variable T : form.
+    Hypothesis T_bounded : bounded 3 T.
+    Hypothesis T_decidable : forall x y k,
+        Qdec (T[num x .: num y .: (num k) ..]).
+    Hypothesis T_sem : forall ρ x y,
+        f x y <-> interp_nat; ρ ⊨ ∃ T[num x .: (num y) ..].
+
+    Definition T' := T ∧ ∀∀ ($1⊕$0 ⧀ $3⊕$4) ~> (¬ $1 == $3) ~> T[$2.:$1.:$0..] ~> ⊥.
+
+
+    Lemma subst_T_bound (ρ : env term) :
+      T[ρ] = T[ρ 0 .: ρ 1 .: (ρ 2) ..].
+    Proof.
+      eapply bounded_subst; first apply T_bounded.
+      intros [|[|[|n]]] H; cbn; lia + easy.
+    Qed.
+    Lemma T_single_rho_model M (I : interp M) ρ x y k :
+      ((iμ k) .: ρ) ⊨ T[num x .: (num y) ..] <-> ρ ⊨ T[num x .: num y .: (num k) ..].
+    Proof.
+      assert (iμ k = eval ρ (num k)) as Hk by (induction k; cbn; congruence).
+      rewrite Hk at 1. rewrite sat_single, subst_comp, subst_T_bound.
+      cbn. rewrite !num_subst. reflexivity.
+    Qed.
+    Lemma T_single_rho_nat ρ x y k :
+      (k .: ρ) ⊨ T[num x .: (num y) ..] <-> ρ ⊨ T[num x .: num y .: (num k) ..].
+    Proof.
+      replace k with (iμ k) at 1; first apply T_single_rho_model.
+      induction k; cbn; congruence.
+    Qed.
+
+    Lemma T_sem' x y ρ :
+      f x y <-> exists k, interp_nat; ρ ⊨ T[num x .: num y .: (num k) ..].
+    Proof.
+      split.
+      - intros H. apply T_sem with (ρ := ρ) in H as [k Hk].
+        exists k. now apply T_single_rho_nat.
+      - intros [k Hk]. eapply T_sem. exists k. apply T_single_rho_nat, Hk.
+    Qed.
+
+
+    Lemma VR1 x y : f x y -> Qeq ⊢C ∃T'[num x .: (num y) ..].
+    Proof.
+      intros Hf. apply completeness.
+      intros M I ρ Mext HI.
+      assert (exists k, (fun _ => 0) ⊨ T[num x .: num y .: (num k) ..]) as [k Hk] by now apply T_sem'.
+      exists (iμ k). split.
+      - apply T_single_rho_model. now eapply dec_completeness; eauto.
+      - intros y' k' [d Hle] Hneq HT. cbn.
+
+        cbn in Hle. rewrite !num_subst, !eval_num, Mext in Hle.
+
+        assert (standard (iμ y i⊕ iμ k)) as Hyk.
+        { rewrite add_hom; try assumption. apply num_standard. }
+        rewrite Hle, !add_rec, <-standard_succ in Hyk; try assumption.
+        apply standard_add in Hyk as [[[y'' <-] [k'' <-]]%standard_add [d' <-]]; try assumption.
+
+        cbn in Hneq. rewrite Mext,!num_subst,eval_num in Hneq.
+        assert (y'' <> y) as Hy''k by congruence.
+
+        rewrite !sat_single_PA, !subst_comp, subst_T_bound in HT. cbn in HT.
+        rewrite !num_subst in HT.
+        eapply dec_completeness with (ρN := fun _ => 0) in HT; try eauto.
+
+        eapply Hy''k, f_func; eapply T_sem'; eauto.
+    Qed.
+    Lemma VR2 x y' y : f x y -> y <> y' -> Qeq ⊢C ¬∃T'[num x .: (num y') ..].
+    Proof.
+      intros Hf Hy. apply completeness.
+      intros M I ρ Mext HI [k [Hk1 Hk2]]. cbn.
+      assert (exists k, (fun _ => 0) ⊨ T[num x .: num y .: (num k) ..]) as [kk Hkk] by now apply T_sem'.
+
+      cbn in Hk2. apply (Hk2 (iμ y) (iμ kk)).
+      - enough (iμ y i⊕ iμ kk i⧀ iμ y' i⊕ k) as [d Hd].
+        { exists d. now rewrite !num_subst, eval_num, Mext.  }
+        rewrite add_hom; try assumption.
+        eapply nonstandard_large; try assumption.
+        enough (~standard k) as Hk.
+        { rewrite standard_add; try assumption. tauto. }
+        intros [ks <-]. apply Hy.
+
+        eapply f_func.
+        + exact Hf.
+        + eapply T_sem' with (ρ := fun _ => 0). exists ks.
+          eapply dec_completeness; eauto. rewrite <-T_single_rho_model.
+          apply Hk1.
+      - rewrite !num_subst, eval_num, Mext. contradict Hy. now eapply iμ_inj.
+      - rewrite !sat_single_PA, !subst_comp, subst_T_bound. cbn. rewrite !num_subst.
+        eapply dec_completeness; eauto.
+    Qed.
+  End value.
+End completeness.
+
+
+Section Qtrichotomy.
+  Existing Instance PA_funcs_signature.
+  Existing Instance PA_preds_signature.
+
+  Lemma Qdec_le x : Q ⊢C ∀ (num x ⧀ σ $0) ∨ ($0 ⧀ σ (num x)).
+  Proof. induction x. Admitted.
+End Qtrichotomy.
+
+Module value_disjoint. Section value_disjoint.
   Existing Instance PA_funcs_signature.
   Existing Instance PA_preds_signature.
 
   Existing Instance class.
 
-  Existing Instance interp_nat.
+  Variable P1 P2 : nat -> Prop.
+  Hypothesis P_disjoint : forall x, P1 x -> P2 x -> False.
+
+  Variable φ1 φ2 : form.
+  Hypothesis (φ1_bounded : bounded 2 φ1) (φ2_bounded : bounded 2 φ2).
+  Hypothesis (φ1_dec : forall x k, Qdec (φ1[num x .: (num k) ..]))
+              (φ2_dec : forall x k, Qdec (φ2[num x .: (num k) ..])).
+  Hypothesis (φ1_sem : forall x, P1 x <-> Qeq ⊢C ∃ φ1[(num x) ..])
+              (φ2_sem : forall x, P2 x <-> Qeq ⊢C ∃ φ2[(num x) ..]).
+
+  Definition φ1' := φ1 ∧ ∀ $0 ⧀ σ $2 ~> φ2[$1 .: $0 ..] ~> ⊥.
+  Definition φ2' := φ2 ∧ ∀ $0 ⧀ σ $2 ~> φ1[$1 .: $0 ..] ~> ⊥.
+  Lemma DR1 x : P1 x -> Qeq ⊢C ∃ φ1'[(num x)..].
+  Proof.
+    admit. (* by Σcompleteness *)
+  Admitted.
+  Lemma DR1' x : P2 x -> Qeq ⊢C ∃ φ2'[(num x)..].
+  Proof.
+    admit. (* by Σcompleteness *)
+  Admitted.
+  Lemma DR2 x : P2 x -> Qeq ⊢C ¬∃ φ1'[(num x)..].
+  Proof.
+    intros Hx%DR1'.
+    cbn -[Qeq]. unfold "↑".
+    apply II. eapply ExE.
+    { eapply Ctx. eauto. }
+    cbn -[Qeq].
+    replace (List.map (subst_form ↑) Qeq) with Qeq by reflexivity.
+    rewrite subst_comp. rewrite (φ2_bounded_subst φ2_bounded). cbn -[Qeq]. rewrite num_subst.
+    eapply Weak.
+    2: { instantiate (1 :=((φ1[(num x)..] ∧ (∀ (∃ σ $2 == σ $1 ⊕ $0) ~> ¬ φ2[num x .: $0..]) :: Qeq))%list).
+         intros ϕ [H|H]; subst.
+         - now left.
+         - now do 2 right. }
+    (* By Sigma1 *)
+    assert (exists k, Qeq ⊢C φ2'[num x .: (num k) ..]) as [k Hk] by admit.
+    cbn -[Qeq] in Hk. rewrite !num_subst in Hk. unfold "↑" in Hk.
+    assert (Qeq ⊢C (num k ⧀ σ $0) ∨ ($0 ⧀ σ (num k))) by admit.
+    eapply DE. { eapply Weak; first apply H. intros ϕ HQ. now right. }
+    - eapply IE.
+      2: { eapply (AllE (num k)). eapply CE2. apply Ctx. right. left. reflexivity. }
+      cbn -[Qeq]. unfold "↑". rewrite num_subst.
+      apply II.
+      eapply IE; first eapply IE.
+      { apply Ctx. left. reflexivity. }
+      + apply Ctx. right. left. reflexivity.
+      + rewrite subst_comp, (φ2_bounded_subst φ2_bounded).  cbn -[Qeq]. rewrite num_subst.
+        eapply Weak. { eapply CE1, Hk. }
+        now do 3 right.
+    - eapply IE.
+      2: { eapply (AllE $0). eapply CE2. eapply Weak; first apply Hk. intros HQ. now do 2 right. }
+      cbn -[Qeq]. unfold "↑". rewrite !num_subst.
+      apply II.
+      eapply IE; first eapply IE.
+      { apply Ctx. left. reflexivity. }
+      + apply Ctx. right. left. reflexivity.
+      + eapply CE1. apply Ctx. do 2 right. left.
+        f_equal. rewrite !subst_comp. eapply bounded_subst.
+        * apply φ1_bounded.
+        * intros [|[|n]] Hn; cbn; rewrite ?num_subst; reflexivity + lia.
+  Admitted.
+End value_disjoint. End value_disjoint.
+
+
+Section Qinsep.
+  Existing Instance PA_funcs_signature.
+  Existing Instance PA_preds_signature.
+
+  Existing Instance class.
+
+  Hypothesis LEM : forall P, P \/ ~P.
 
   Hypothesis completeness : forall φ,
-    Qeq ⊢C φ <-> forall (M : Type) (I : interp M) ρ, extensional I -> I ⊨=L Qeq -> ρ ⊨ φ.
-  Hypothesis Σcompleteness : forall M (I : interp M) φ ρN ρM,
-      bounded 0 φ -> Σ1 φ ->
-      interp_nat, ρN ⊨ φ ->
-      I, ρM ⊨ φ.
-  Hypothesis Δ0decidability : forall φ, Δ0' φ -> Qeq ⊢C φ \/ Qeq ⊢C ¬φ.
+      Qeq ⊢C φ <-> forall (M : Type) (I : interp M) ρ, extensional I -> I ⊨=L Qeq -> ρ ⊨ φ.
 
-  Variable f : nat -> nat -> option nat.
-  Variable f_func : forall x y1 y2 k1 k2, f x k1 = Some y1 -> f x k2 = Some y2 -> y1 = y2.
+  Variable theta : nat -> nat -> nat -> option bool.
+  Hypothesis theta_stationary : forall c, fstationary (theta c).
+  Hypothesis theta_univ : forall (f : nat -> nat -> option bool), fstationary f ->
+            exists c, forall x y, freturns f x y <-> freturns (theta c) x y.
+  Arguments theta_univ : clear implicits.
 
-  Variable T : form.
-  Hypothesis T_bounded : bounded 3 T.
-  (* NOTE Delta1 could suffice here, since its still decidable *)
-  Hypothesis T_Δ0 : Δ0' T.
-  Hypothesis T_sem : forall M (I : interp M) ρ x y,
-      (exists k, f x k = Some y) <-> ρ ⊨ ∃ T[num x .: (num y) ..].
-  (* T is functional in nat. This assumption is implicit in the post by saying "a T predicate",
-     I guess *)
-  Hypothesis T_func : forall ρ x k k' y y',
-      interp_nat, ρ ⊨ T[num x .: num y .: (num k) ..] ->
-      interp_nat, ρ ⊨ T[num x .: num y' .: (num k') ..] ->
-      y = y' /\ k = k'.
-  Hypothesis T_syn : forall x y,
-      (exists k, f x k = Some y) <-> Qeq ⊢C ∃ T[num x .: num y .: $0 ..].
+  Hypothesis Qrepr : forall P, enumerable P -> exists φ,
+        bounded 2 φ /\ (forall x k, Qdec φ[num x .: (num k) ..]) /\
+          forall x ρ, P x <-> interp_nat; ρ ⊨ ∃φ[(num x)..].
 
-  Definition T' := T ∧ ∀∀ ($1⊕$0 ⧀ $3⊕$4) ~> T[$2.:$1.:$0..] ~> ⊥.
-
-  Lemma sat_T_bound M (I : interp M) (ρ : env M) :
-    ρ ⊨ T <-> (ρ 0 .: ρ 1 .: ρ 2 .: (fun _ => iO)) ⊨ T.
+  Local Definition P b := fun t => let '(c, x) := unembed t in freturns (theta c) x b.
+  Local Lemma P_enumerable b :
+    enumerable (P b).
   Proof.
-    split.
-    - eapply bound_ext; first apply T_bounded.
-      intros [|[|[|n]]] H; cbn; lia + easy.
-    - eapply bound_ext; first apply T_bounded.
-      intros [|[|[|n]]] H; cbn; lia + easy.
+    apply semi_decidable_enumerable.
+    { exists Some. eauto. }
+    unfold semi_decidable.
+    exists (fun t k => let '(c, x) := unembed t in match theta c x k with
+                                          | Some true =>
+                                              if b then true else false
+                                          | Some false =>
+                                              if b then false else true
+                                          | _ => false
+                                          end).
+    intros t. unfold P. destruct (unembed t) as [x y]; split; intros [k Hk].
+    - exists k. destruct b; now rewrite Hk.
+    - exists k. now destruct b, (theta x y k) as [[]|].
   Qed.
-  Lemma subst_T_bound (ρ : env term) :
-    T[ρ] = T[ρ 0 .: ρ 1 .: (ρ 2) ..].
+  Local Lemma P_disjoint t : P true t -> P false t -> False.
   Proof.
-    eapply bounded_subst; first apply T_bounded.
-    intros [|[|[|n]]] H; cbn; lia + easy.
+    unfold P. destruct (unembed t) as [x y].
+    intros [k1 Hk1] [k2 Hk2].
+    assert (k1 >= k2 \/ k2 >= k1) as [H|H] by lia.
+    - specialize (theta_stationary Hk2 H). congruence.
+    - specialize (theta_stationary Hk1 H). congruence.
   Qed.
 
-  Lemma sat_subst_single_nat φ (ρ : env nat) (k : nat) :
-    (k .: ρ) ⊨ φ -> ρ ⊨ φ [(num k)..].
+  Lemma Qincomplete : exists φ, ~Qeq ⊢C φ /\ ~Qeq ⊢C ¬φ.
   Proof.
-    rewrite <-sat_single, eval_num.
-    replace (iμ k) with k; first easy.
-    induction k; cbn; congruence.
+    unshelve edestruct guess_insep_expl_incompleteness as (s & Hs1 & Hs2).
+    - exact theta.
+    - apply Qfs_class, LEM.
+    - apply theta_univ.
+    - destruct (Qrepr (P_enumerable true)) as (φ1 & Hb1 & Hd1 & Hr1),
+               (Qrepr (P_enumerable false)) as (φ0 & Hb0 & Hd0 & Hr0).
+
+      unshelve eexists.
+      { intros c x. exists (∃ (φ1' φ1 φ0)[(num (embed (c, x)))..]). apply bounded_closed.
+        constructor. eapply subst_bound; first eapply φ1'_bounded; first assumption.
+        intros [|[|n]] H; cbn.
+        + eapply bounded_up_t; first apply num_bound. lia.
+        + constructor. lia.
+        + lia. }
+
+      split.
+      + intros c x Hx. cbn -[φ1' φ2']. unfold form_provable, CT.Q. cbn [proj1_sig form_neg].
+        exists Qeq. split; first easy.
+        eapply DR1. 2: exact P_disjoint. all: try assumption.
+        unfold P. now rewrite embedP.
+      + intros c x Hx. cbn -[φ1' φ2']. unfold form_provable, CT.Q. cbn [proj1_sig form_neg].
+        exists Qeq. split; first easy.
+        eapply DR2. 2: exact P_disjoint. all: try assumption.
+        unfold P. now rewrite embedP.
+    - destruct s as [φ Hc]. exists φ.
+      split.
+      + contradict Hs1. now exists Qeq.
+      + contradict Hs2. now exists Qeq.
   Qed.
-  Lemma sat_subst_single_model M (I : interp M) φ (ρ : env M) (k : nat) :
-    (iμ k .: ρ) ⊨ φ <-> ρ ⊨ φ[(num k)..].
-  Proof.
-    split.
-    - intros H. rewrite <-sat_single. now rewrite eval_num.
-    - intros H. rewrite <-sat_single in H.
-      now rewrite eval_num in H.
-  Qed.
-
-  Lemma T_completeness M (I : interp M) (Mext : extensional I) (MQ : I ⊨=L Qeq) ρN ρM x y k :
-    interp_nat, ρN ⊨ T[num x .: num y .: (num k) ..] <-> I, ρM ⊨ T[num x .: num y .: (num k)..].
-  Proof.
-    split.
-    - intros H. eapply Σcompleteness.
-      + eapply subst_bound; first apply T_bounded.
-        intros [|[|[|n]]]; intros H'; last lia.
-        all: apply num_bound.
-      + admit.
-      + apply H.
-    - intros H. destruct Δ0decidability with (φ := T[num x .: num y .: (num k) ..]) as [HQ|HQ].
-      + admit. (* TODO by substitution *)
-      + eapply completeness; now auto using nat_is_Q_model.
-      + eapply completeness with (I := I) in HQ; try assumption.
-        exfalso. apply HQ, H.
-  Admitted.
-  Lemma T_single_rho_model M (I : interp M) ρ x y k :
-     ((iμ k) .: ρ) ⊨ T[num x .: (num y) ..] <-> ρ ⊨ T[num x .: num y .: (num k) ..].
-  Proof.
-    assert (iμ k = eval ρ (num k)) as Hk by (induction k; cbn; congruence).
-    rewrite Hk at 1. rewrite sat_single, subst_comp, subst_T_bound.
-    cbn. rewrite !num_subst. reflexivity.
-  Qed.
-  Lemma T_single_rho_nat ρ x y k :
-     (k .: ρ) ⊨ T[num x .: (num y) ..] <-> ρ ⊨ T[num x .: num y .: (num k) ..].
-  Proof.
-    replace k with (iμ k) at 1; first apply T_single_rho_model.
-    induction k; cbn; congruence.
-  Qed.
-
-  Lemma T_sem' x y ρ :
-    (exists k, f x k = Some y) <-> exists k, interp_nat, ρ ⊨ T[num x .: num y .: (num k) ..].
-  Proof.
-    split.
-    - intros H. eapply T_sem with (I := interp_nat) (ρ := ρ) in H.
-      destruct H as [k Hk]. exists k. now apply T_single_rho_nat.
-    - intros [k Hk]. eapply T_sem. exists k. apply T_single_rho_nat, Hk.
-  Qed.
-
-
-  Lemma VR1 x y : (exists k, f x k = Some y) -> Qeq ⊢C ∃T'[num x .: (num y) ..].
-  Proof.
-    intros Hf. apply completeness.
-    intros M I ρ Mext HI.
-    assert (exists k, (fun _ => 0) ⊨ T[num x .: num y .: (num k) ..]) as [k Hk] by now apply T_sem'.
-    exists (iμ k). split.
-    - apply T_single_rho_model. now eapply T_completeness, Hk.
-    - intros y' k' [d Hle] HT. cbn.
-      cbn in Hle. rewrite !num_subst, !eval_num, Mext in Hle.
-
-      assert (standard (iμ y i⊕ iμ k)) as Hyk.
-      { rewrite add_hom; try assumption. apply num_standard. }
-      rewrite Hle, !add_rec, <-standard_succ in Hyk; try assumption.
-      apply standard_add in Hyk as [[[y'' <-] [k'' <-]]%standard_add [d' <-]]; try assumption.
-
-      assert (y + k = S y'' + k'' + d') as Hle'.
-      { eapply iμ_inj; try assumption. cbn.
-        rewrite <-!add_hom, <-add_rec; try assumption. }
-
-      rewrite !sat_subst_single_model, !subst_comp, subst_T_bound in HT. cbn in HT.
-      rewrite !num_subst in HT.
-      eapply T_completeness in HT; try assumption.
-
-      pose proof (T_func Hk HT). lia.
-  Qed.
-  Lemma VR2 x y' y : (exists k, f x k = Some y) -> y <> y' -> Qeq ⊢C ¬∃T'[num x .: (num y') ..].
-  Proof.
-    intros Hf Hy. apply completeness.
-    intros M I ρ Mext HI [k [Hk1 Hk2]]. cbn.
-    assert (exists k, (fun _ => 0) ⊨ T[num x .: num y .: (num k) ..]) as [kk Hkk] by now apply T_sem'.
-
-    cbn in Hk2. apply (Hk2 (iμ y) (iμ kk)).
-    - enough (iμ y i⊕ iμ kk i⧀ iμ y' i⊕ k) as [d Hd].
-      { exists d. now rewrite !num_subst, eval_num, Mext.  }
-      rewrite add_hom; try assumption.
-      eapply nonstandard_large; try assumption.
-      enough (~standard k) as Hk.
-      { rewrite standard_add; try assumption. tauto. }
-      intros [ks <-]. apply Hy.
-
-      assert (exists k, f x k = Some y').
-      { eapply T_sem' with (ρ := fun _ => 0). exists ks.
-        rewrite T_completeness, <-T_single_rho_model; first apply Hk1; assumption. }
-
-      destruct Hf, H.
-      eapply f_func; eassumption.
-    - rewrite !sat_subst_single_model, !subst_comp, subst_T_bound. cbn.
-      rewrite !num_subst.
-      eapply T_completeness, Hkk; try assumption.
-  Qed.
-End value.
+End Qinsep.
+Check Qincomplete.
 
 
 Section value.
@@ -477,4 +806,3 @@ Section value.
   Qed.
 
 End value.
-Check VR_total.
